feat(HPKE): WIP: Spec for mode Base is complete
Some type refinements for length limits are still missing.

specs/Spec.Agile.HPKE.fsti
@@ -73,20 +73,21 @@ let max_psk (cs:ciphersuite): size_nat = pow2 16 - 1
 
 // TODO rename? length of what? plaintext, right?
 inline_for_extraction
-let max_length (cs:ciphersuite) : size_nat = AEAD.max_length (aead_of_cs cs)
+let max_length (cs:ciphersuite):size_nat = AEAD.max_length (aead_of_cs cs)
 
 // TODO This could be refined depending on the underlying hash function?
 inline_for_extraction
-let max_pskID: size_nat = pow2 16 - 1
+let max_pskID (cs:ciphersuite):size_nat = pow2 16 - 1
 
 // TODO This could be refined depending on the underlying hash function?
 inline_for_extraction
-let max_info: size_nat = pow2 16 - 1
+let max_info (cs:ciphersuite):size_nat = pow2 16 - 1
 
 // TODO This could be refined depending on the underlying hash function?
 inline_for_extraction
 let max_exp_ctx: size_nat = pow2 16 - 1
 
+let max_seq (cs:ciphersuite): nat = pow2 (8*(size_aead_nonce cs)) - 1
 
 
 /// Types
@@ -96,23 +97,62 @@ type key_dh_secret_s (cs:ciphersuite) = lbytes (size_dh_key cs)
 type key_kem_s (cs:ciphersuite) = lbytes (size_kem_key cs) // TODO This is true for the current DHKEM. It would be nice to have it modular depending on the KEM.
 type key_aead_s (cs:ciphersuite) = lbytes (size_aead_key cs)
 type nonce_aead_s (cs:ciphersuite) = lbytes (size_aead_nonce cs)
+type seq_aead_s (cs:ciphersuite) = n:nat{n <= max_seq cs}
 type psk_s (cs:ciphersuite) = b:bytes{Seq.length b <= max_psk cs}
+type pskID_s (cs:ciphersuite) = b:bytes{Seq.length b <= max_pskID cs}
 type exporter_secret_s (cs:ciphersuite) = lbytes (size_kdf cs)
-type info_s (cs:ciphersuite) = b:bytes{Seq.length b <= max_info} // TODO should this be _s?
+type info_s (cs:ciphersuite) = b:bytes{Seq.length b <= max_info cs} // TODO should this be _s?
 type exp_ctx_s (cs:ciphersuite) = b:bytes{Seq.length b <= max_exp_ctx} // TODO should this be _s?
 
-let encryption_context (cs:ciphersuite) = key_aead_s cs & nonce_aead_s cs & nat & exporter_secret_s cs
+// TODO can we hide the contents of encryption_context, i.e. not
+//      expose them in this fsti, to avoid usage which is not
+//      conform with the spec?
+let encryption_context (cs:ciphersuite) = key_aead_s cs & nonce_aead_s cs & seq_aead_s cs & exporter_secret_s cs
+
+val context_export:
+    cs:ciphersuite
+  -> ctx:encryption_context cs
+  -> exp_ctx:exp_ctx_s cs // TODO replace this by a pre-condition that uses labeled_expand predicates
+  -> l:size_nat ->
+  Pure (lbytes l)
+    (requires HKDF.expand_output_length_pred (hash_of_cs cs) l)
+    (ensures fun _ -> True)
+
+val context_compute_nonce:
+    cs:ciphersuite
+  -> ctx:encryption_context cs
+  -> seq:seq_aead_s cs ->
+  Tot (nonce_aead_s cs)
+
+val context_increment_seq:
+    cs:ciphersuite
+  -> ctx:encryption_context cs ->
+  Tot (option (encryption_context cs))
+
+val context_seal:
+    cs:ciphersuite
+  -> ctx:encryption_context cs
+  -> aad:AEAD.ad (aead_of_cs cs)
+  -> pt:AEAD.plain (aead_of_cs cs) ->
+  Tot (option (encryption_context cs & AEAD.cipher (aead_of_cs cs)))
+
+val context_open:
+    cs:ciphersuite
+  -> ctx:encryption_context cs
+  -> aad:AEAD.ad (aead_of_cs cs)
+  -> ct:AEAD.cipher (aead_of_cs cs) ->
+  Tot (option (encryption_context cs & AEAD.plain (aead_of_cs cs)))
 
 val setupBaseS:
     cs:ciphersuite
   -> skE:key_dh_secret_s cs
-  -> pkR:key_dh_public_s cs
+  -> pkR:DH.serialized_point (curve_of_cs cs)
   -> info:info_s cs ->
   Tot (option (key_dh_public_s cs & encryption_context cs))
 
 val setupBaseR:
     cs:ciphersuite
-  -> pkE:key_dh_public_s cs
+  -> enc:key_dh_public_s cs
   -> skR:key_dh_secret_s cs
   -> info:info_s cs ->
   Tot (option (encryption_context cs))
@@ -120,7 +160,7 @@ val setupBaseR:
 val sealBase:
     cs:ciphersuite
   -> skE:key_dh_secret_s cs
-  -> pkR:key_dh_public_s cs
+  -> pkR:DH.serialized_point (curve_of_cs cs)
   -> info:info_s cs
   -> aad:AEAD.ad (aead_of_cs cs)
   -> pt:AEAD.plain (aead_of_cs cs) ->
@@ -135,10 +175,3 @@ val openBase:
   -> ct:AEAD.cipher (aead_of_cs cs) ->
   Tot (option (AEAD.decrypted #(aead_of_cs cs) ct))
 
-val context_export:
-    cs:ciphersuite
-  -> ctx:encryption_context cs
-  -> exp_ctx:exp_ctx_s cs
-  -> l:nat ->
-  // TODO Inside HKDF, l is restricted to <= 255 hash lengths. Need to repeat here? No: because HPKE does not have this limitation itself? Would it be better to reflect the limitation here by using some variable exposed by HKDF, like we do with AEAD above?
-  Tot (option (lbytes (size_kdf cs)))
